assignments/chapter04/exercise02.dfy
@@ -12,8 +12,14 @@ include "chapter03-exercise03.dfy"
 /*}*/
 ghost predicate Inv(c:Constants, v:Variables) {
 /*{*/
-  true  // Replace me: probably not strong enough. :v)
-/*}*/
+   v.WellFormed(c) && (
+    (v.server == (true, -1) &&
+     (forall i:nat | i < |v.clientsHoldingLock| :: !v.clientsHoldingLock[i]))
+    ||
+    (!v.server.0 && 0 <= v.server.1 < c.clients &&
+     (forall i:nat | i < |v.clientsHoldingLock| :: v.clientsHoldingLock[i] ==> i == v.server.1))
+  )
+  /*}*/
 }
 
 // Here's your obligation. Probably easiest to break this up into three
@@ -24,5 +30,10 @@ lemma SafetyTheorem(c:Constants, v:Variables, v':Variables)
   ensures Inv(c, v) ==> Safety(c, v)
 {
 /*{*/
+  assert Init(c, v) ==> Inv(c, v);
+  assert forall i:nat | i<|v.clientsHoldingLock| :: Inv(c, v) && Release(c, v, v', i) ==> Inv(c, v');
+  assert forall i:nat | i<|v.clientsHoldingLock| :: Inv(c, v) && Acquire(c, v, v', i) ==> Inv(c, v');
+  // assert Inv(c, v) && Acquire(c, v, v', 0) ==> Inv(c, v');
+  assert Inv(c, v) && Next(c, v, v') ==> Inv(c, v');
 /*}*/
 }
