demos/chapter04/crawler-v2.dfy
@@ -1,0 +1,55 @@
+datatype Variables = Variables(y:int, isGoingNorth: bool)
+
+predicate Init(v: Variables){
+    && v.y == 5
+    && v.isGoingNorth
+}
+
+predicate MoveNorth(v:Variables, v':Variables){
+    && v.isGoingNorth
+    && v' == v.(y := v.y + 1)
+}
+
+predicate MoveSouth(v:Variables, v':Variables){
+    && !v.isGoingNorth
+    && v' == v.(y := v.y - 1)
+}
+
+predicate Flip(v:Variables, v':Variables){
+    && v'.y + v.y == 0
+    && v'.isGoingNorth != v.isGoingNorth
+}
+
+predicate Next(v:Variables, v':Variables){
+    || MoveNorth(v, v')
+    || MoveSouth(v, v')
+    || Flip(v, v')
+}
+
+predicate Safety(v:Variables){
+    && v.y*v.y > 9
+}
+
+predicate Inv(v:Variables){
+    (v.y >= 5 && v.isGoingNorth) || (v.y <= -5 && !v.isGoingNorth)
+}
+lemma InvImpliesSafety(v:Variables)
+    requires Inv(v)
+    ensures Safety(v)
+{
+}
+
+lemma InitImpliesInv(v:Variables)
+    requires Init(v)
+    ensures Inv(v)
+{
+
+}
+
+lemma NextMaintainsInv(v:Variables, v':Variables)
+    requires Inv(v)
+    requires Next(v, v')
+    ensures Inv(v')
+{
+
+}
