demos/chapter04/leader-election.dfy
@@ -1,0 +1,116 @@
+datatype Constants = Constants(ids: seq<nat>){
+    ghost predicate ValidIdx(i:nat){
+        i < |ids|
+    }
+
+    ghost predicate WellFormed(){
+        1 < |ids|
+    }
+    ghost predicate UniqueIds(){
+        forall i, j | 
+        && 0 <= i < |ids|
+        && 0<= j < |ids| 
+        && ids[i] == ids[j] :: i == j
+    }
+    ghost function getNextID(actor:nat): nat {
+        if actor == |ids|-1 then 0 else actor+1
+    }
+}
+
+datatype Variables = Variables(max_seen: seq<int>) {
+    ghost predicate WellFormed(c: Constants){
+        && c.WellFormed()
+        && |max_seen| == |c.ids|
+    }
+}
+
+ghost predicate Init(c: Constants, v: Variables){
+    && v.WellFormed(c)
+    && c.UniqueIds()
+    && forall i:nat | c.ValidIdx(i) :: v.max_seen[i] == -1
+}
+
+ghost function max(a:int, b:int) : (ret:int)
+    ensures ret == a || ret == b
+    ensures ret >= a && ret >= b 
+{
+    if a < b then b else a
+}
+
+ghost predicate Update(c:Constants, v:Variables, v': Variables, actor: nat){
+    && c.ValidIdx(actor)
+    && v.WellFormed(c)
+    && var nextActor := c.getNextID(actor);
+    && var msg := max(c.ids[actor], v.max_seen[actor]);
+    && v'.max_seen == v.max_seen[nextActor := max(msg, v.max_seen[nextActor])]
+}
+
+datatype Step = UpdateStep(actor:nat)
+
+ghost predicate NextStep(c:Constants, v:Variables, v':Variables, step:Step){
+    match step 
+        case UpdateStep(actor) => Update(c,v,v',actor)
+}
+
+ghost predicate Next(c:Constants, v:Variables, v':Variables){
+    exists step:Step :: NextStep(c,v,v',step)
+}
+
+ghost predicate IsLeader(c:Constants, v:Variables, actor:nat){
+    && c.ValidIdx(actor)
+    && v.WellFormed(c)
+    && v.max_seen[actor] == c.ids[actor]
+}
+
+ghost predicate Safety(c:Constants, v:Variables){
+    // && v.WellFormed(c)
+    && forall i: nat, j:nat | c.ValidIdx(i) && c.ValidIdx(j) && IsLeader(c,v,i) && IsLeader(c,v,j) :: i==j
+}
+
+ghost predicate InBetween(start:nat, mid:nat, end:nat){
+    if start > end then
+        mid > start || mid < end
+    else  start < mid < end
+}
+
+ghost predicate ChordDominates(c:Constants, v:Variables){
+    && v.WellFormed(c)
+    && (forall start:nat, mid:nat, end:nat | 
+        && c.ValidIdx(start) 
+        && c.ValidIdx(mid)
+        && c.ValidIdx(end)
+        && v.max_seen[end] == c.ids[start]
+        && InBetween(start, mid, end) 
+            :: c.ids[mid] < c.ids[start]
+        )
+}
+
+ghost predicate Inv(c:Constants, v:Variables){
+    // && v.WellFormed(c)
+    && Safety(c,v)  
+    // && c.UniqueIds()
+    && ChordDominates(c,v)
+}
+
+lemma InvImpliesSafety(c:Constants, v: Variables) 
+    requires Inv(c, v)
+    ensures Safety(c, v)
+{   
+}
+
+lemma InitImpliesInv(c:Constants, v: Variables)
+    requires Init(c, v)
+    ensures Inv(c, v)
+{
+    assert v.WellFormed(c);
+    assert c.UniqueIds();
+  
+}
+
+lemma NextPreservesInv(c:Constants, v: Variables, v': Variables) 
+    requires Inv(c, v)
+    requires Next(c, v, v')
+    ensures Inv(c, v')
+{
+    assert Inv(c,v');
+}
